::: {.content-hidden}
$$
{{< include macros.tex >}}
$$
:::




# Preliminaries

Before introducing $\R$ we want to make sure that we cover all the basics needed for the task.



## Sets

A sets is a **collection** of objects. These objects are called **elements** of the set. For example in the previous section we mentioned the following sets:

- $\N$ the set of natural numbers
- $\Z$ the set of integers
- $\Q$ the set of rational numbers
- $\R$ the set of real numbers

Given an arbitrary set $A$, we write 
$$
x \in A
$$ 

if the element $x$ belongs to the set $A$. If an element $x$ is not contained in $A$, we say that 

$$
x \notin A \,.
$$

::: Remark

A set can contain all sorts of elements. For example the students in a classroom can be modelled by a set $S$. The elements of the set are the students. For example

$$
S = \{ 
    \text{Alice, Olivia, Jake, Sahab}   
     \}
$$

In this case we have

$$
\text{Alice} \in S 
$$
but instead

$$
\text{Silvio} \notin S \,. 
$$

:::




## Logic

In this section we introduce some basic logic symbols. Suppose that you are given two statements, say $\alpha$ and $\beta$. The formula
$$
\alpha \implies \beta
$$
means that $\alpha$ **implies** $\beta$. In other words, if $\alpha$ is true then also $\beta$ is true.  
The formula
$$
\alpha \impliedby \beta
$$
means that $\alpha$ is implied by $\beta$: if $\beta$ is true then also $\alpha$ is true.  
When we write
$$
\alpha \iff \beta
$$ {#eq-iff}
we mean that $\alpha$ and $\beta$ are **equivalent**. Note that (@eq-iff) is equivalent to 
$$
\alpha \implies \beta  \,\, \text{ and } \,\,
\beta \implies \alpha \,.
$$
Such equivalence is very useful in proofs.

::: Example
We have that 
$$
x > 0 \implies x>-100 \,,
$$
and 
$$
\text{ contradiction }   \impliedby  \sqrt{2} \in \Q \,.
$$
Concerning $\iff$ we have
$$
x^2 < 2  \iff  - \sqrt{2} < x < \sqrt{2} \,.
$$
:::

We now introduce logic **quantifiers**. These are 

* $\forall$ which reads **for all**
* $\exists$ which reads **exists**
* $\exists !$ which reads **exists unique**
* $\not\exists$ which reads **does not exists**

These work in the following way. Suppose that you are given a statement $\alpha(x)$ which depends on the point $x \in \R$. Then we say 

* $\alpha(x)$ is satisfied for all $x \in A$ with $A$ some collection of numbers. This translates to the symbols
$$
\alpha(x) \, \text{ is true } \, \forall \, x \in A \,,
$$
* There exists some $x$ in $\R$ such that $\alpha(x)$ is satisfied: in symbols
$$
\exists \, x \in \R \, \text{ such that } \, \alpha(x) \, \text{ is true},
$$
* There exists a unique $x_0$ in $\R$ such that $\alpha(x)$ is satisfied: in symbols
$$
\exists ! \, x_0 \in \R \, \text{ such that } \, \alpha(x_0) \, \text{ is true},
$$
* $\alpha(x)$ is never satisfied: 
$$
\not\exists  \, x \in \R \, \text{ such that } \, \alpha(x) \, \text{ is true}.
$$


::: Example

Let us make concrete examples:

* The expression $x^2$ is always non-negative. Thus we can say
$$
x^2 \geq 0 \,\, \text{ for all } \,\, x \in \R \,.
$$
* The equation $x^2=1$ has two solutions $x=1$ and $x=-1$. Therefore we can say
$$
\exists \, x \in \R \, \text{such that } \, x^2  = 1 \,. 
$$
* The equation $x^3=1$ has a unique solution $x=1$. Thus
$$
\exists ! \, x \in \R \, \text{such that } \, x^3  = 1 \,. 
$$
* We know that the equation $x^2=2$ has no solutions in $\Q$. Then
$$
\not\exists  \, x \in \Q \, \text{such that } \, x^2  = 2 \,. 
$$
:::







## Operations on sets

### Union and intersection

For two sets $A$ and $B$ we define their **union** as the set
$$
A \cup B := \{ x\, \colon \, x \in A  \, \text{ or } \, x \in B \} \,.
$$
The **intersection** of $A$ and $B$ is defined by
$$
A \cap B := \{ x\, \colon \, x \in A  \, \text{ and } \, x \in B \} \,.
$$
We denote the **empty set** by the symbol $\emptyset$. Two sets are **disjoint** if 
$$
A \cap B = \emptyset \,.
$$

::: Example

Define the subset of rational numbers
$$
S:= \left\{ x \in \Q \, \colon \, 0 < x < \frac52 \right\} \,.
$$
Then we have 
$$
\N \cap S = \{1, 2 \} \,.
$$
We can also define the sets of **even** and **odd** numbers by 

\begin{align}
E & := \{ 2n \, \colon \, n \in \N \} \,,\\
O & := \{ 2n+1 \, \colon \, n \in \N \} \,.
\end{align}

Then we have

\begin{align}
\N \cap E & = E \,, \,\, \N \cap O = O \,, \\
O \cup E & = \N \,, \,\, O \cap D = \emptyset \,.
\end{align}

:::




### Inclusion and equality


Given two sets $A$ and $B$, we say that $A$ is **contained** in $B$ if all the elements of $A$ are also contained in $B$. This will be denoted with the **inclusion** symbol $\subset$, that is,
$$
A \subset B \,.
$$
In this case we say that 

- $A$ is a **subset** of $B$, 
- $B$ is a **superset** of $A$.

The inclusion $A \subset B$ is equivalent to the implication:
$$
x \in A \,\, \implies \,\, x \in B 
$$
for all $x \in A$. The symbol $\implies$ reads **implies**, and denotes the fact that the first condition implies the second.


::: Example

Given two sets $A$ and $B$ we always have
\begin{gather}
(A \cap B) \subset A \,, \,\, (A \cap B) \subset B \,,\\
A \subset (A \cup B) \,, \,\, B \subset (A \cup B) \,.
\end{gather}

:::


We say that two sets $A$ and $B$ are equal if they contain the **same** elements. We denote equality by the symbol
$$
A=B \,.
$$


::: Example

The sets 
$$
A =\{ 1,2,3 \}
$$
and 
$$
B= \{ 3 ,1,2\}
$$
are equal. This is because they contain exactly the same elements: **order** does not matter when talking about sets. 

:::

::: {.Proposition #Proposition-Equality-Sets}

Let $A$ and $B$ be sets. Then 
$$
A=B
$$
**if and only if**
$$
A \subset B \,\, \text{ and } \,\, B \subset A \,.
$$

:::



::: Proof
The proof is almost trivial. However it is a good exercise in basic logic, so let us do it. 


1. First implication $\implies$:  
Suppose that $A=B$. Let us show that $A\subset B$. Since $A = B$, this means that all the elements of $A$ are also contained in $B$. Therefore if we take $x \in A$ we have
$$
x \in A \,\, \implies \,\, x \in B \,.
$$
This shows $A \subset B$. The proof of $B \subset A$ is similar. 

2. Second implication $\impliedby$:  
Suppose that $A \subset B$ and $B \subset A$. We need to show $A=B$, that is, $A$ and $B$ have the same elements. To this end let $x \in A$. Since $A \subset B$ then we have $x \in B$. Thus $B$ contains all the elements of $A$. Since we are also assuming $B \subset A$, this means that $A$ contains all the elements of $B$. Hence $A$ and $B$ contain the same elements, and $A=B$.

:::


The above proposition is very useful when we need to **prove** that two sets are equal: rather than showing directly that $A = B$, we can prove that $A \subset B$ and $B \subset A$. 




### Infinite unions and intersections

Suppose given a set $\Omega$, and a family of sets $A_n \subset \Omega$, where $n \in \N$. Then we can define the **infinte union**
$$
\bigcup_{n \in \N} A_n := \{ x \in \Omega \, \colon \, x \in A_n \,\, \text{ for at least one } \,\, n \in \N \} \,.
$$
The **infinte intersection** is defined as
$$
\bigcap_{n \in \N} A_n := \{ x \in \Omega \, \colon \, x \in A_n \,\, \text{ for all } \,\, n \in \N \} \,.
$$

::: Example 

Let the ambient set be $\Omega:=\N$ and define the family $A_n$ by
\begin{align}
A_1 & := \{ 1, 2, 3 , 4 , \ldots \} \\
A_2 & := \{ 2, 3 , 4 , 5, \ldots \} \\
A_3 & := \{ 3 , 4 , 5, 6, \ldots \} \\
& \ldots \ldots  \\
A_n & := \{ n, n+1, n+2, n+3,  \ldots \} \,,
\end{align}
for arbitrary $n \in \N$. Then
$$
\bigcup_{n \in \N} A_n = \N \,.
$$ {#eq-infinite-union}
The above equality can be easily proven using Proposition \ref{Proposition-Equality-Sets}. Indeed, assume that $m \in \cup_n A_n$. Then $m \in A_n$ for at least one $n \in \N$. Since $A_n \subset \N$, we conclude that $m \in \N$. This shows 
$$
\bigcup_{n \in \N} A_n \subset \N \,.
$$
Conversely, suppose that $m \in \N$. By definition $m \in A_m$. Hence there exists at least one index $n$, $n=m$ in this case, such that $m \in A_n$. Then by definition $m \in \cup_{n \in \N} A_n$, showing that
$$
\N \subset \bigcup_{n \in \N} A_n \,.
$$
Hence we conclude (@eq-infinite-union) by Proposition \ref{Proposition-Equality-Sets}.  
We also have that
$$
\bigcap_{n \in \N} A_n = \emptyset \,.
$$ {#eq-infinite-intersection}
We prove the above by **contradiction**. Indeed, suppose that (@eq-infinite-intersection) is false, i.e., 
$$
\bigcap_{n \in \N} A_n \neq \emptyset \,.
$$
This means there exists some $m \in \N$ such that $m \in \cap_{n \in \N} A_n$. Hence, by definition, $m \in A_n$ for all $n \in \N$. However $m \notin A_{m+1}$, yielding a contradiction. Thus (@eq-infinite-intersection) holds.
:::




### Complement

Suppose that $A$ and $B$ are subsets of a larger set $\Omega$. The **complement** of $A$ with respect to $B$ is the set of elements of $B$ which do not belong to $A$, that is
$$
B \smallsetminus A := \{ x \in \Omega \, \colon \, x \in B \, \text{ and } \, x \notin A \} \,.
$$
In particular, the complement of $A$ with respect to $\Omega$ is denoted by 
$$
A^c := \Omega \smallsetminus A := \{ x \in \Omega \, \colon \, x \notin A \} \,.
$$


::: Remark

Suppose that $A \subset \Omega$. Then $A$ and $A^c$ form a **partition** of $\Omega$, in the sense that
$$
A \cup A^c = \Omega  \,\, \text{ and } \,\,  A \cap A^c = \emptyset \,.
$$

:::

::: Example

Suppose $A, B \subset \Omega$. Then
$$
A \subset B  \iff B^c \subset A^c \,.
$$

Let us prove the above claim:

- First implication $\implies$:  
Suppose that $A \subset B$. We need to show that $B^c \subset A^c$. Hence, assume $x \in B^c$. By definition this means that $x \notin B$. Now notice that we cannot have that $x \in A$. Indeed, assume $x \in A$.  By assumption we have $A \subset B$, hence $x \in B$. But we had assumed $x \in B$, contradiction. Therefore it must be that $x \notin A$. Thus $B^c \subset A^c$.

- Second implication $\impliedby$:  
Essentially the same proof, hence we omit it.  
:::

We conclude by stating the De Morgan's Laws. The proof will be left as an exercise.

::: Proposition
## De Morgan's Laws

Suppose $A,B \subset \Omega$. Then
$$
(A \cap B)^c = A^c \cup B^c 
$$
and
$$
(A \cup B)^c = A^c \cap B^c  \,.
$$ 

:::



### Product of sets

Suppose $A$ and $B$ are two sets. The **product** of $A$ and $B$ is the set of pairs
$$
A \times B := \{ (a,b) \, \colon \, a \in A, \, b \in B \} \,.
$$
By definition two elements in $A \times B$ are the same, in symbols
$$
(a, b) = (\tilde{a}, \tilde{b})
$$
if and only if they are equal component-by-componenent, that is
$$
a=\tilde{a}\,, \qquad b = \tilde{b} \,.
$$




## Equivalence relation


Suppose $A$ is a set. A **binary relation** $R$ on $A$ is a subset 
$$
R \subset A \times A \,.
$$

::: Definition
### Equivalence relation

A binary relation $R$ is called an **equivalence relation** if it satisfies the following properties:

1. **Reflexive**: For each $x \in A$ one has 
$$
(x,x) \in R \,, 
$$

    > This is saying that all the elements in $A$ must be related to themselves

2. **Symmetric**: We have
$$
(x,y) \in R \implies (y,x) \in R
$$

    > If $x$ is related to $y$, then $y$ is related to $x$

3. **Transitive**: We have
$$
(x,y) \in R \,, \,\, (y,z) \in R  \implies (x,z) \in R 
$$

    > If $x$ is related to $y$, and $y$ is related to $z$, then $x$ must be related to $z$


If $(x,y) \in R$ we write
$$
x \sim y 
$$
and we say that $x$ and $y$ are **equivalent**.
:::





::: Definition
### Equivalence classes

Suppose $R$ is an **equivalence relation** on $A$. The **equivalence class** of an element $x \in A$ is the set
$$
[x]:=\{ y \in A \, \colon \, y \sim x \} \,.
$$
The set of equivalence classes of elements of $A$ with respect to the equivalence relation $R$ is denoted by 
$$
A / R \, :=  \,\{ [x] \, \colon \, x \in A \} \,.
$$


:::


Let us immediately clarify the above definitions by considering the prototypical example of equivalence relation: the **equality**.


::: Example
### Equality is an equivalence relation

Consider the set of natural numbers $\N$. The equality defines a **binary relation** on $\N \times \N$, via
$$
R:=\{ (x,y) \in \N \times \N \, \colon \, x=y  \} \,.
$$
Let us check that $R$ is an **equivalence relation**:

1. Reflexive: It holds, since $x=x$ for all $x \in \N$,

2. Symmetric: Again $x = y$ if and only if $y = x$,

3. Transitive: If $x = y$ and $y = z$ then $x = z$.

The class of equivalence of $x \in \N$ is given by
$$
[x] = \{ x \}\,,
$$
that is, this relation is quite trivial, given that each element of $\N$ can only be related to itself. The quotient space is then 
$$
\N / R = \{ [x] \divider x \in \N \} = \{  \{ x\} \divider x \in \N \}  \,.
$$
:::




::: Example
Suppose that $R$ is a binary relation on the set $\Q$ of rational numbers defined by
$$
x \sim y  \iff x-y \in \Z \,.
$$
Then $R$ is an equivalence relation on $\Q$. Indeed:

1. Reflexive: Let $x \in \Q$. Then $x-x = 0$ and $0 \in \Z$. Thus $x \sim x$.
2. Symmetric: If $x \sim y$ then $x-y \in \Z$. But then also  
$$
-(x-y) = y - x \in \Z
$$
and so $y \sim x$.
3. Transitive: Suppose $x \sim y$ and $y \sim z$. Then 
$$
x - y \in \Z \,  \text{ and } \, y - z \in \Z \,.
$$
Thus we have
$$
x-z = (x-y) + (y-z) \in \Z
$$
showing that $x \sim z$. This shows that $R$ is an equivalence relation on $\Q$.


Now note that 
$$
y \sim x \iff y -x \in \Z 
$$
and the above is equivalent to
$$
\exists \, n \in \Z \, \text{ s.t. } \, y - x = n
$$
which again is equivalent to 
$$
\exists \, n \in \Z \, \text{ s.t. } \, y = x + n \,.
$$
Therefore all the elements of $\Q$ related to $x$ by $R$ are of the form 
$$
x + n \,, \, \forall \, n \in \Z \,.
$$
The equivalence classes with respect to $R$ are then
$$
 [x] = \{  x + n \ \colon \ n \in \Z  \}  \,.
$$
Each equivalence class has exactly one element in $[0,1) \cap \Q$, meaning that:
$$
\forall x \in \Q \,, \,\, \exists! \, q \in \Q \st  0 \leq q < 1 \, \text{ and } \, q \in [x]\,.
$$
Therefore 
$$
\Q / R = \{ [x] \divider x \in \Q \} = \{ q \in \Q \divider 0 \leq q <1  \} \,.
$$
:::





## Order relation

Similarly, we define **order relations**.


::: Definition
### Order relation

A binary relation $R$ is called an **order relation** if it satisfies the following properties:

1. **Reflexive**: For each $x \in A$ one has 
$$
(x,x) \in R \,, 
$$

2. **Transitive**: We have
$$
(x,y) \in R \,, \,\, (y,z) \in R  \implies (x,z) \in R 
$$


3. **Antisymmetric**: We have
$$
(x,y) \in R \,  \text{ and } \, (y,x) \in R \implies x = y 
$$

    > This is the only new condition with respect to the definition of equivalence relation. 

:::


The prototypical example of order relation is the **inequality** relation.


::: Example
### Inequality is an order relation

Consider the set of integers $\Z$. The inequality defines a **binary relation** on $\Z \times \Z$, via
$$
R:=\{ (x,y) \in \Z \times \Z \, \colon \, x \leq y  \} \,.
$$
Let us check that $R$ is an **order relation**:

1. Reflexive: It holds, since $x \leq x$ for all $x \in \Z$,

2. Transitive: If $x \leq y$ and $y \leq z$ then $x \leq z$.

3. Antisymmetric: If $x \leq y$ and $y \leq x$  then $x = y$.

:::





## Intervals

In this section we assume to have available the set $\R$ of **real numbers**, which we recall is an extension of $\Q$. We now introduce the concept of **interval**.

::: Definition

Let $a,b \in \R$ with $a<b$. We define the **open interval** $(a,b)$ as the set
$$
(a,b) := \{ x \in \R \, \colon \, a < x < b \}\,.
$$
We define the **close interval** $[a,b]$ as the set
$$
[a,b] := \{ x \in \R \, \colon \, a \leq x \leq b \}\,.
$$
:::

In general we also define the intervals
\begin{align}
[a,b) & := \{ x \in \R \, \colon \, a \leq x < b \}\,, \\
(a,b] & := \{ x \in \R \, \colon \, a \leq x \leq b \}\,, \\
(a, \infty) & := \{ x \in \R \, \colon \, x > a  \}\,, \\
[a, \infty) & := \{ x \in \R \, \colon \, x \geq a  \}\,, \\
(-\infty, b) & := \{ x \in \R \, \colon \, x < b  \}\,, \\
(-\infty, b] & := \{ x \in \R \, \colon \, x \leq b  \}\,.
\end{align}

Some of the above intervals are depicted in @fig-interval-1, @fig-interval-2, @fig-interval-3, @fig-interval-4 below. 

![Interval $(a,b)$](/images/interval_1.png){#fig-interval-1 width=60%}

![Interval $[a,b]$](/images/interval_2.png){#fig-interval-2 width=60%}

![Interval $(a,\infty)$](/images/interval_3.png){#fig-interval-3 width=60%}

![Interval $(-\infty,b]$](/images/interval_4.png){#fig-interval-4 width=60%}






## Absolute value or Modulus

In this section we assume to have available the set $\R$ of **real numbers**, which we recall is an extension of $\Q$. 

::: Definition
### Absolute value 
For $x \in \R$ we define its **absolute value** as the quantity
$$
|x| = 
\begin{cases}
x  & \text{ if } \, x \geq 0 \\
-x  & \text{ if } \, x < 0 
\end{cases}
$$
:::

::: Example

By definition one has $|x|=x$ if $x \geq 0$. For example
$$
|\pi| = \pi \,, \,\, \left|\sqrt{2}\right| = \sqrt{2} \,, \,\, |0|=0 \,.
$$
Instead $|x|= -x$ if $x < 0$. For example 
$$
|-\pi| = \pi \,, \,\, \left|-\sqrt{2}\right| = \sqrt{2} \,, \,\, |-10|=10 \,.
$$
:::


Let us also make the following basic remark, whose proof will be left as an exercise.

::: Remark
For all $x \in \R$ one has 
$$
|x| \geq 0 \,.
$$
Moreover 
$$
|x| = 0 \iff x = 0 \,.
$$
:::

Another basic remark (proof by exercise).

::: {.Remark #rmk-absolute-value-sym}

For all $x \in \R$ one has
$$
|x| = |-x| \,.
$$

:::


You might be familiar with the graph associated to the absolute value function:

![Plot of the absolute value function $f(x)=|x|$](/images/absolute_value.png){width=40%}


However in these Lecture Notes we are not dealing with functions, so it is better to think about the absolute value in a geometric way.  





::: Remark
### Geometric interpretation of $|x|$
A number $x \in \R$ can be represented with a point on the real line $\R$.The non-negative number $|x|$ represents the **distance** of $x$ from the origin $0$. Notice that this works for both positive and negative numbers $x_1$ and $x_2$ respectively, as shown in @fig-absolute-value-1 below.
:::


![Geometric interpretation of $|x|$](/images/absolute_value_1.png){#fig-absolute-value-1 width=70%}



::: Remark
### Geometric interpretation of $|x-y|$

If $x,y \in \R$ then the number $|x-y|$ represents the distance between $x$ and $y$ on the real line, as shown in @fig-absolute-value-2 below.
Note that by Remark \ref{rmk-absolute-value-sym} we have
$$
|x-y| = |y-x| \,.
$$
:::

![Geometric interpretation of $|x-y|$](/images/absolute_value_2.png){#fig-absolute-value-2 width=70%}


In the next Lemma we show a fundamental equivalence regarding the absolute value.

::: {.Lemma #lemma-absolute-value}
Let $x,y \in \R$. Then
$$
|x| \leq y  \iff -y \leq x \leq y \,.
$$
:::

The geometric meaning of the above statement is clear: the distance of $x$ from the origin is less than $y$, in formulae 
$$
|x| \leq y\,,
$$
if and only if $x$ belongs to the interval $[-y,y]$, in formulae
$$
-y \leq x \leq y \,.
$$ 
A sketch of this explanation is seen in @fig-absolute-value-3 below.

![Geometric meaning of Lemma \ref{lemma-absolute-value}](/images/absolute_value_3.png){#fig-absolute-value-3 width=70%}


::: Proof
### Proof of Lemma \ref{lemma-absolute-value}

We divide the proof in steps.  

* Step 1: implication $\implies$  
Suppose first that 
$$
|x| \leq y \,.
$$ {#eq-lemma-absolute-value-1}
Recalling that the absolute value is non-negative, from (@eq-lemma-absolute-value-1) we deduce that $0 \leq |x| \leq y$. In particular it holds 
$$
y \geq 0 \,.
$$ {#eq-lemma-absolute-value-2}
We make separate arguments for the cases $x \geq 0$ and $x<0$:

    - Case 1: $x \geq 0$.  From (@eq-lemma-absolute-value-1), (@eq-lemma-absolute-value-2) and from $x \geq 0$ we have
    $$
    -y \leq 0 \leq x = |x| \leq y
    $$
    which shows 
    $$
    -y \leq x \leq y \,.
    $$
    - Case 2: $x < 0$. From (@eq-lemma-absolute-value-1), (@eq-lemma-absolute-value-2) and from $x < 0$ we have
    $$
    -y \leq 0 < - x = |x| \leq y
    $$
    which shows 
    $$
    -y \leq - x \leq y \,.
    $$
    Multiplying the above inequalities by $-1$ yields
    $$
    -y \leq x \leq y \,.
    $$

* Step 2: implication $\impliedby$  
Suppose now that  
$$
-y \leq x \leq  y \,.
$$ {#eq-lemma-absolute-value-3}
We make separate arguments for the cases $x \geq 0$ and $x<0$:

    - Case 1: $x \geq 0$. Since $x \geq 0$, from (@eq-lemma-absolute-value-3) we get
    $$
    |x| = x \leq y
    $$
    showing that 
    $$
    |x| \leq y \,.
    $$
    - Case 2: $x < 0$. Since $x < 0$, from (@eq-lemma-absolute-value-3) we have
    $$
    -y \leq x = - |x| \,.
    $$
    Multiplying the above inequality by $-1$ yields
    $$
    |x| \leq y \,.
    $$
:::


With basically the same arguments, one can also show the following.


::: Lemma
Let $x,y \in \R$. Then
$$
|x| < y  \iff -y < x < y \,.
$$
:::




## Triangle inequality

The triangle inequality relates the absolute value to the sum operation. It is a very important inequality, which we will use a lot in the future.

::: Theorem
### Triangle inequality  {#theorem-triangle-inequality}

For every $x, y \in \R$ we have
$$
| |x| - |y| | \leq |x-y| \leq |x| + |y| \,.
$$ {#eq-triangle-inequality}
:::


Before proceeding with the proof, let us discuss the geometric meaning of the triangle inequality.



::: Remark
### Geometric meaning of triangle inequality

The notion of absolute value can be extended also to vectors in the plane. Suppose that $x$ and $y$ are two vectors in the plane, as in @fig-triangle-ineq-1 below. Then $|x|$ and $|y|$ can be interpreted as the **lengths** of these vectors.  
Using the rule of sum of vectors, we can draw $x+y$, as shown in @fig-triangle-ineq-2 below. From the picture it is evident that 
$$
|x+y| \leq |x| + |y|\,,
$$ {#eq-triangle-inequality-1}
that is, *the length of each side of a triangle does not exceed the sum of the lengths of the two remaining sides*. Note that (@eq-triangle-inequality-1) is exactly the second inequality in (@eq-triangle-inequality). This is why (@eq-triangle-inequality) is called triangle inequality.
:::


![Vectors $x$ and $y$](/images/triangle_ineq_1.png){#fig-triangle-ineq-1 width=20%}


![Summing the vectors $x$ and $y$. The triangle inequality relates the length of $x+y$ to the length of $x$ and $y$](/images/triangle_ineq_2.png){#fig-triangle-ineq-2 width=35%}





::: Proof
### Proof of Theorem \ref{theorem-triangle-inequality}

Assume that $x,y \in \R$. We prove the two inequalities in (@eq-triangle-inequality) individually.

- Proof of the second inequality in (@eq-triangle-inequality):  
Trivially we have
$$
|x| \leq |x| \,.
$$
Therefore we can apply Lemma \ref{lemma-absolute-value} and infer
$$
-|x| \leq x \leq |x| \,.
$$ {#eq-triangle-inequality-3}
Similarly we have that $|y| \leq |y|$, and so Lemma \ref{lemma-absolute-value} implies
$$
-|y| \leq y \leq |y| \,.
$$ {#eq-triangle-inequality-4}
Summing (@eq-triangle-inequality-3) and (@eq-triangle-inequality-4) we get
$$
-(|x| + |y|) \leq x + y \leq |x| + |y| \,.
$$
We can now again apply Lemma \ref{lemma-absolute-value} to get
$$
|x + y| \leq |x| + |y| \,,
$$ {#eq-triangle-inequality-5}
which is the second inequality in (@eq-triangle-inequality).

- Proof of the second inequality in (@eq-triangle-inequality):  
Note that the trivial identity
$$
x = x+y - y
$$
always holds. We then have
\begin{align}
|x| & = |x+y - y| \\
    & = |(x+y) + (-y)| \\
    & = |a+b|
\end{align}
with $a=x+y$ and $b=-y$. We can now apply (@eq-triangle-inequality-5) to $a$ and $b$ to obtain
\begin{align}
|x| & = |a+b| \\
    & \leq |a| + |b| \\
    & = |x+y| + |-y| \\
    & = |x+y| + |y|
\end{align}
Therefore
$$
|x| - |y| \leq |x+y| \,.
$$ {#eq-triangle-inequality-6}
We can now swap $x$ and $y$ in (@eq-triangle-inequality-6) to get
$$
|y| - |x| \leq |x+y| \,.
$$
By rearranging the above inequality we obtain
$$
-|x+y| \leq |x| - |y|  \,.
$$ {#eq-triangle-inequality-7}
Putting together (@eq-triangle-inequality-6) and (@eq-triangle-inequality-7) yields
$$
-|x+y| \leq |x| - |y| \leq |x+y| \,.  
$$
By Lemma \ref{lemma-absolute-value} the above is equivalent to
$$
||x| - |y|| \leq |x+y| \,,
$$
which is the first inequality in (@eq-triangle-inequality).
:::



An immediate consequence of the triangle inequality are the following inequalities, which are left as an exercise. 



::: Remark
For any $x,y \in \R$ it holds
$$
||x|-|y|| \leq |x-y| \leq |x|+|y|\,.
$$
Moreover for any  $x,y,z \in \R$ it holds
$$
|x-y| \leq |x-z| + |z-y| \,.
$$
:::





## Proofs involving $\e$





## Induction





## Example: Approximating $\sqrt{2}$


