::: {.content-hidden}
$$
{{< include macros.tex >}}
$$

:::


# Real Numbers


In this chapter we introduce the sysyem of Real Numbers $\R$. 


## Fields

In order to introduce $\R$, we need the concepts of **binary operation** and **field**. We proceed in a general setting, starting from a set $K$.


::: Definition
### Binary operation
A binary operation on a set $K$ is a function 
$$
\circ \ \colon K \times K \to K
$$
which maps the ordered pair $(x,y)$ into $x \circ y$.
:::


::: Notation
There are two main binary operations we are interested in:

- **Addition**: denoted by $+$. The addition, or **sum** of $x,y \in K$ is denoted by 
$$
x + y \,.
$$
- **Multiplication**: denoted by $\cdot$. The multiplication, or **product** of $x,y \in K$ is denoted by 
$$
x \cdot y \,\, \mbox{ or } \,\, xy\,.
$$
:::


::: Example
### of binary operation  {#example-binary-operation}

Let $K=\{0,1\}$. We can for example define the operations of sum and product according to the tables 
$$
\begin{array}{c|cc}
 + & 0 & 1 \\ \hline
 0 & 0 & 1 \\
 1 & 1 & 0 \\
\end{array}	
\qquad \qquad
\begin{array}{c|cc}
\cdot & 0 & 1 \\ \hline
    0 & 0 & 0 \\
    1 & 0 & 1 \\
\end{array}
$$
The above mean that 
$$
0+0 = 1+1 = 0 \,, \quad 0 + 1 = 1 + 0 = 1\,, 
$$
$$
0 \cdot 0 = 0 \cdot 1 = 1 \cdot 0 = 0 \,, \quad 1 \cdot 1 = 1  \,.
$$
This is just one option. Note that we could not have defined 
$$
1 + 1  = 2\,,
$$
since $2 \notin K$.
:::

Binary operations take ordered pairs of elements of $K$ as input. Therefore the operation
$$
x \circ y \circ z
$$
does not make sense, since we do not know which one between
$$
x \circ y  \,\, \mbox{ or } \,\, y \circ z
$$
has to be performed first. Also one could have that the outcome of an operation depends on order:
$$
x \circ y \neq y \circ x \,.
$$
This motivates the following definition. 


::: Definition
Let $K$ be a set and $\circ \ \colon K \times K \to K$ be a binary operation on $K$. We say that:

1. $\circ$ is **commutative** if $\forall \, x,y \in K$
    $$
    x \circ y = y \circ x \,.
    $$
2. $\circ$ is **associative** if $\forall \, x,y,z \in K$
    $$
    (x \circ y) \circ z = x \circ (y \circ z) \,.
    $$
3. An element $e \in K$ is called **neutral element** of $\circ$ if $\forall \, x \in K$
    $$ 
    x \circ e = e \circ x = e \,.
    $$
4. Let $e$ be a neutral element of $\circ$ and let $x \in K$. An element $y \in K$ is called an **inverse** of $x$ with respect to $\circ$ if 
$$
x \circ y = y \circ x = e \,.
$$
:::


::: {.Example #example-binary-operation-2}

Let $K$ with $+$ and $\cdot$ be as in Example \ref{example-binary-operation}. For the sum we have

- $+$ is commutative, since 
$$
0 + 1 = 1 + 0 = 0 \,.  
$$
- $+$ is associative, since for example 
$$
(0 + 1) + 1 = 1 + 1 = 0 \,, \quad 0 + (1 + 1) = 0 + 0 = 0 \,,  
$$
and therefore 
$$
(0 + 1) + 1 = 0 + (1 + 1) \,.
$$
In general one can show that $+$ is associative by checking all the other permutations. 
- The neutral element of $+$ is $0$, since 
$$
0 + 0 = 0 \,, \quad 1 + 0 = 0 + 1 = 1 \,.
$$
- Every element has an inverse. Indeed, the inverse of $0$ is $0$, since 
$$
0 + 0 = 0\,,
$$
while the inverse of $1$ is $1$, since
$$
1 + 1 = 1 + 1 = 0 \,.
$$

For the product we have:

- $\cdot$ is commutative, since 
$$
1 \cdot 0 = 0 \cdot 1 = 0 \,.
$$
- $\cdot$ is associative, since for example 
$$
(0 \cdot 1) \cdot 1 = 0 \cdot 1 = 0 \,, \quad 0 \cdot (1 \cdot 1) = 0 \cdot 1 = 0 \,,  
$$
and therefore 
$$
(0 \cdot 1) \cdot 1 = 0 \cdot (1 \cdot 1) \,.
$$
By checking all the other permutations one can show that $\cdot$ is associative.
- The neutral element of $\cdot$ is $1$, since 
$$
0 \cdot 1 = 1 \cdot 0 = 0 \,, \quad 1 \cdot 1 =  1 \,.
$$
- The element $0$ has no inverse, since  
$$
0 \cdot 0 = 0 \cdot 1 = 1 \cdot 0 = 0\,,
$$
and thus we never obtain the neutral element $1$. The inverse of $1$ is given by $1$, since 
$$
1 \cdot 1 = 1 \,.
$$
:::


::: Example
Let $K=\{0,1\}$ be a set with binary relation $\circ$ defined by the table
$$
\begin{array}{c|cc}
 \circ & 0 & 1 \\ \hline
 0     & 1 & 1 \\
 1     & 0 & 0 \\
\end{array}	
$$
In this case $\circ$ is not commutative since 
$$
0 \circ 1 = 1 \, , \quad 1 \circ 0 = 0
$$
and therefore
$$
0 \circ 1 \neq 1 \circ 0 \,.
$$
Moreover $\circ$ is not associative, since 
$$
(0 \circ 1) \circ 1 = 1 \circ 1 = 0 \,,
$$
while 
$$
0 (\circ 1 \circ 1) = 0 \circ 0 = 1 \,.
$$

:::


We are ready to define fields.


::: Definition
### Field

Let $K$ be a set with binary operations $+$ and $\cdot$. We call the triple $(K, + , \cdot)$ a **field** if:

1. The addition $+$ satisfies:
    - (A1) $+$ is **commutative** and **associative**.
    - (A2) There exists a **neutral element** in $K$ for $+$. We call this element $0$. 
    - (A3) For every $x \in K$ there exists an inverse $y \in K$ with respect to $+$. We call this element the **additive inverse** of $x$ and denote it by $y=-x$.
2. The multiplication $\cdot$ satisfies:
    - (M1) $\cdot$ is **commutative** and **associative**.
    - (M2) There exists a **neutral element** in $K$ for $\cdot$. We call this element $1$. 
    - (M3) For every $x \in K$ with $x \neq 0$ there exists an inverse $y \in K$ with respect to $\cdot$. We call this element the **multiplciative inverse** of $x$ and denote it by $y=x^{-1}$.
3. $+$ and $\cdot$ are related by the **distributive property**:
    - (AM) For all $x,y,z \in K$ we have
    $$
    x \cdot (y + z) = (x \cdot y) + (y \cdot z) \,.
    $$
:::


::: Example
Let $K$ with $+$ and $\cdot$ be as in Example \ref{example-binary-operation}. We can show that $(K,+,\cdot)$ is a field. Indeed we have already shown in Example \ref{example-binary-operation-2} that: 

- (A1) and (M1) hold, 
- (A2) holds with neutral element $0$,
- (M2) holds with neutral element $1$,
- (A3) every element has an additive inverse, with
$$
-0 = 0 \,, \quad - 1 = 1 \,,
$$
- (M3) every element which is not $0$ a multiplicative inverse, with
$$
1^{-1} = 1\,.
$$
- (AM) this is left to show: Indeed, for all $y,z \in K$ we have
$$
0 \cdot (y + z) = 0 \,, \quad (0 \cdot y) + (0 \cdot z) = 0 + 0 = 0\,,
$$
and also
$$
1 \cdot (y + z) = y + z \,, \quad (1 \cdot y) + (1 \cdot z) = y + z \,.
$$
:::


::: Definition
### Subtraction and division
Let $(K,+,\cdot)$ be a field. We define:

- **Subtraction** as the operation $-$ defined by 
$$
x - y := x + (-y) \,, \quad \forall \, x , y \in K \,,
$$
where $-y$ is the additive inverse of $y$.
- **Division** as the operation $/$ defined by
$$
x/y := x \cdot y^{-1}\,, \quad \forall \, x , y \in K \,, \,\, y \neq 0 \,,
$$
where $y^{-1}$ is the multiplicative inverse of $y$.
:::



::: Proposition
### Uniqueness of neutral elements and inverses

Let $(K,+,\cdot)$ be a field. Then

1. There is a unique element in $K$ with the property of $0$,
2. There is a unique element in $K$ with the property of $1$,
3. For all $x \in K$ there is a unique additive inverse $-x$,
4. For all $x \in K$, $x \neq 0$, there is a unique multiplicative inverse $x^{-1}$.
:::

::: Proof
1. Suppose that $0 \in K$ and $\tilde{0} \in K$ are both neutral element of $+$, that is, they both satisfy (A2). Then 
$$
0 + \tilde{0} = 0
$$
since $\tilde{0}$ is a neutral element for $+$. Moreover
$$
\tilde{0} + 0 = \tilde{0}
$$
since $0$ is a neutral element for $+$. By commutativity of $+$, see property (A1), we have
$$
0 = 0 + \tilde{0} = \tilde{0} + 0 = \tilde{0} \,,
$$
showing that $0 = \tilde{0}$. Hence the neutral element for $+$ is unique.
2. Exercise.
3. Let $x \in K$ and suppose that $y, \tilde{y} \in K$ are both additive inverses of $x$, that is, they both satisfy (A3). Therefore
$$
x + y = 0
$$
since $y$ is an additive inverse of $x$ and
$$
x + \tilde{y} = 0 
$$
since $\tilde{y}$ is an additive inverse of $x$. Therefore we can use commutativity and associativity and of $+$, see property (A1), and the fact that $0$ is the neutral element of $+$, to infer
\begin{align}
y & = y + 0 = y + (x + \tilde{y}) \\ 
  & = (y + x) + \tilde{y} = (x + y) + \tilde{y} \\
  & = 0 + \tilde{y} = \tilde{y} \,,    
\end{align}
concluding that $y = \tilde{y}$. Thus there is a unique additive inverse of $x$, and 
$$
y = \tilde{y} = -x \,,
$$
with $-x$ the element from property (A3).
4. Exercise.
:::



Using the properties of field we can also show that the usual properties of sum, subtraction, multiplication and division still hold in any field. We list such properties in the following proposition.


::: Proposition
### Properties of field operations
Let $(K,+,\cdot)$ be a field. Then for all $x,y,z \in K$,

- $x + y = x + z \,\, \implies \,\, y = z$
- $x \cdot y = x \cdot z \,$ and $\,x \neq 0 \,\, \implies \,\, y = z$
- $- 0 = 0$
- $1^{-1} = 1$
- $x \cdot 0 = 0$
- $-1 \cdot x = -x$
- $-(-x) = x$
- $(x^{-1})^{-1} = x \,$ if $\, x \neq 0$
- $(x \cdot y)^{-1} = x^{-1} \cdot y^{-1}$ 
:::




The above properties can be all proven with elementary use of the field properties (A1)-(A3), (M1)-(M3) and (AM). This is an exercise in patience, and is left to the reader.



Let us conclude with examining the sets of numbers introduced in @sec-chap-1. 

::: Theorem
Consider the sets $\N$, $\Z$, $\Q$ with the usual operations $+$ and $\cdot$. We have:

- $(\N, + , \cdot)$ is **not a field**:  
It satisfies properties (A1), (A2), (M1), (M2), (AM) of fields. It is missing properties (A3) and (M3), the additive and multiplicative inverse properties, respectively.
- $(\Z, + , \cdot)$ is **not a field**:  
It satisfies properties (A1), (A2), (A3), (M1), (M2), (AM) of fields. Thus it is only missing (M3), the multiplicative inverse property.
- $(\Q, + , \cdot)$ **is a field**.


:::

The proof is omitted. 




## Cut Property  

We have just introduced the notion of **field**, and noted that the set of rational numbers with the usual operations
$$
(\Q, + , \cdot)
$$
is a **field**. 

We now need to address the key issue we proved in @sec-chap-1, that is, that
$$
\sqrt{2} \notin \Q \,.
$$
This means that $\Q$ has **gaps**, and cannot be represented as a **continuous** line. The rigorous definition of **lack of gaps** needs the concept of **cut** of a set.



::: Definition
### Partition of a set

Let $S$ be a set. The pair $(A,B)$ is a **partition** of $S$ if
$$
A , B \subset S\,, \quad  A \neq \emptyset\,, \quad B \neq \emptyset \,,
$$
and
$$
S = A \cup B \,, \quad 
A \cap B = \emptyset \, . 
$$
:::



![Schematic picture of partition](/images/partition.png){width=55%}


::: Definition
### Cut of a set

Let $S$ be a set with a total order relation $\leq$. The pair $(A,B)$ is a **cut** of $S$ if 

1. $(A,B)$ is a **partition** of $S$,
2. We have
$$
a \leq b \,,  \quad \forall \, a \in A \,, \,\, \forall \, b \in B \,.
$$
:::

The **cut** of a set is often called **Dedekind cut**, named after **Richard Dedekind**, who used cuts to give an explicit construction of the real numbers $\R$, see [Wikipedia page](https://en.wikipedia.org/wiki/Dedekind_cut).


::: Definition 
### Cut property
Let $S$ be a set with a total order relation $\leq$. We say that $S$ has the **cut property** if for every cut $(A,B)$ of $S$ there exists some $s \in S$ such that 
$$
a \leq s \leq b \,, \quad \forall  \, a \in A\,, \,\, \forall  \, b \in B \,.
$$
We call $s$ the **separator** of the cut $(A,B)$.
:::




::: Example
Let $S = \Q$ and consider the sets
$$
A = (-\infty,s] \cap \Q \,, \quad B = (0,\infty) \cap \Q \,. 
$$
for some $s \in \Q$. Then the pair $(A,B)$ is a cut of $\Q$, and $s$ is the separator.
:::


![$(A,B)$ is a cut of $\Q$ with separator $s$.](/images/cut.png){width=70%}


::: Question
Do all cuts of $\Q$ have a **separator**? In other words, does $\Q$ have the **cut property**?
:::


The answer to the above question is **NO**. For example the pair
$$
A =  (-\infty,\sqrt{2}) \cap \Q \,, \quad B = (\sqrt{2},\infty) \cap \Q\,.
$${#eq-cut-Q}
is a cut of $\Q$, since $\sqrt{2} \notin \Q$. However what is the separator? It should be $s = \sqrt{2}$, given that clearly 
$$
a \leq \sqrt{2}  \leq b \,, \quad \forall \, a \in A\,, \,\, \forall \, b \in B \,.
$$
However $\sqrt{2} \notin \Q$, so we are **NOT ALLOWED** to take it as separator. Indeed, we can show that $(A,B)$ defined as in (@eq-cut-Q) has no separator.



![$(A,B)$ is a cut of $\Q$ which has no separator](/images/cut_sqrt2.png){width=70%}







::: Theorem
### $\Q$ does not have the cut property.

$\Q$ does not have the cut property. More explicitly, there exist a cut $(A,B)$ of $\Q$ which has no separator.
:::

::: Proof
Let $A$ and $B$ be the sets defined in (@eq-cut-Q). It is useful to rewrite $A$ and $B$ in the form
$$
A = A_1 \cup A_2 \,, 
$$
where 
$$
A_1 = \{ q \in \Q \divider q< 0  \}\,, 
$$
$$
A_2 =\{ q \in \Q \divider q \geq 0\,, \,\, q^2 < 2  \} \,,
$$
and
$$
B = \{ q \in \Q \divider q > 0, \,\, q^2 > 2  \} \,.
$$

*Step 1. $(A,B)$ is a cut of $\Q$*:  
We need to prove the following:

1. $(A,B)$ is a partition of $\Q$. This is because $A , B \subset \Q$ with $A \neq \emptyset$ and $B \neq \emptyset$. Moreover 
$A \cap B = \emptyset$ and
$$
A \cup B = \Q\,,
$$ 
given that $\sqrt{2} \notin \Q$, and so there is no element $q \in \Q$ such that $q^2 = 2$.
2. It holds
$$
a \leq b \,, \quad \forall a \in A \,, \,\, \forall \, b \in B \,.
$$
Indeed, suppose that $a \in A$ and $b \in B$. We have two cases:
    - $a \in A_1$: Therefore $a<0$. In particular
    $$
    a < 0 < b\,,
    $$
    given that $b > 0$ for all $b \in B$. Thus $a<b$.
    - $a \in A_2$: Therefore $a \geq 0$ and $a^2 < 2$. In particular
    $$
    a^2 < 2 < b^2 \,,
    $$
    since $b^2>2$ for all $b \in B$. In particular 
    $$
    a^2 < b^2 \,.
    $$
    Since $b>0$ for all $b \in B$, from the above inequality we infer $a<b$, concluding.



*Step 2. $(A,B)$ has no separator*:  
Suppose by contradiction that $(A,B)$ admits a separator
$$
L \in \Q \,.
$$
By definition this means
$$
a \leq L \leq b \,, \quad \forall a \in A \,, \,\, \forall \, b \in B \,.
$${#eq-separator-contradiction}
Since
$$
L \in \Q \,, \quad \Q = A \cup B \,, \quad  A \cap B = \emptyset \,,
$$
then either $L \in A$ or $L \in B$. We will see that both these possibilities lead to a contradiction:

*Case 1: $L \in A$.*  
By (@eq-separator-contradiction) we know that 
$$
a \leq L \,, \quad \forall \, a \in A \,.
$${#eq-separator-contradiction-hp-0}
In particular the above implies 
$$
L \geq 0
$${#eq-separator-contradiction-1}
since $0 \in A$. Therefore we must have $L \in A_2$, that is, 
$$
L \geq 0 \,\, \mbox{ and } \,\, L^2 < 2 \,.
$${#eq-separator-contradiction-hp-1}
Set 
$$
\tilde{L} := L + \frac1n
$$
for $n \in \N$, $n \neq 0$ to be chosen later. Clearly we have
$$
\tilde{L} \in \Q   \,\,\, \mbox{ and } \,\,\, L < \tilde{L}  \,. 
$${#eq-separator-contradiction-2}
From (@eq-separator-contradiction-1) and (@eq-separator-contradiction-2) we have also
$$
\tilde{L}>0 \,.
$${#eq-separator-contradiction-3}
We now want to show that there is a choice of $n$ such that $\tilde{L}^2 < 2$, which will lead to a contradiction. Indeed, we can estimate
\begin{align}
\tilde{L}^2 & = \left( L + \frac1n \right)^2 \\
            & = L^2 + \frac{1}{n^2} + 2 \frac{L}{n} \\
            & < L^2 + \frac{1}{n} + 2 \frac{L}{n}   \qquad  \left(\mbox{using } \, \frac{1}{n}<\frac{1}{n^2}  \right) \\
            & = L^2 + \frac{2L + 1}{n} \,. 
\end{align}
If we now impose that 
$$
L^2 + \frac{2L + 1}{n} < 2 \,,
$$
we can rearrange the above and obtain
$$
n(2 - L^2) > 2L + 1 \,.
$$
Now note that $L^2 < 2$ by assumption (@eq-separator-contradiction-hp-1). Thus we can divived by $(2 - L^2)$ and obtain
$$
n >\frac{2L + 1}{2 - L^2} \,.
$$
Therefore we have just shown that 
$$
n >\frac{2L + 1}{2 - L^2}  \,\, \implies \,\, \tilde{L}^2 < 2 \,.
$$
Together with (@eq-separator-contradiction-3) this implies $\tilde{L} \in A$. Therefore we have
$$
\tilde{L} \leq L
$$
by (@eq-separator-contradiction-hp-0). On the other hand it also holds 
$$
\tilde{L} > L
$$
by (@eq-separator-contradiction-2), and therefore we have a contradiction. Thus $L \notin A$.

*Case 2: $L \in B$.*  
As $L \in B$, we have by definition
$$
L > 0 \,, \quad L^2 > 2 \,.
$${#eq-separator-contradiction-5}
Moreover since $L$ is a separator, see (@eq-separator-contradiction), in particular
$$
L \leq b \,,  \,\, \forall \, b \in B \,.
$${#eq-separator-contradiction-6}
Define now 
$$
\tilde{L} := L - \frac1n
$$
with $n \in \N$, $n \neq 0$ to be chosen later. Clearly we have
$$
\tilde{L} < L \,.
$${#eq-separator-contradiction-7}
We now show that $n$ can be chosen so that $\tilde{L} \in B$. Indeed
\begin{align}
\tilde{L}^2  & = \left(  L - \frac1n   \right)^2 \\
             & = L^2 + \frac{1}{n^2} - 2 \frac{L}{n} \\
             & > L^2 - \frac{1}{n^2} - 2 \frac{L}{n}   \qquad  \left(\mbox{using } \, \frac{1}{n^2} > - \frac{1}{n^2}  \right) \\
             & > L^2 - \frac{1}{n} - 2 \frac{L}{n}   \qquad  \left(\mbox{using } \, -\frac{1}{n^2} > - \frac{1}{n}  \right) \\
             & = L^2 - \frac{1 + 2L}{n} \,.
\end{align}
Now we impose 
$$
L^2 - \frac{1 + 2L}{n} > 2 
$$
which is equivalent to 
$$
n(L^2 - 2) > 1 + 2L \,.
$$
Since we are assuming $L \in B$, then $L^2 > 2$, see (@eq-separator-contradiction-5). Therefore we can divide by $(L^2 -2)$ and get
$$
n > \frac{1+2L}{L^2 - 2} \,.
$$
In total, we have just shown that 
$$
 n > \frac{1+2L}{L^2 - 2} \quad \implies \quad \tilde{L}^2 > 2\,,
$$
proving that $\tilde{L} \in B$. Therefore by (@eq-separator-contradiction-6) we get
$$
L \leq \tilde{L} \,.
$$
This contradicts (@eq-separator-contradiction-7).

*Conclusion:*  
We have seen that assuming that $(A,B)$ has a separator $L \in \Q$ leads to a contradiction. Thus the cut $(A,B)$ has no separator.
:::


::: Remark

The above proof can be summarized by saying that the set
$$
A = (-\infty, \sqrt{2}) \cap \Q
$$
does not admit a **largest** element in $\Q$, and that the set
$$
B = (\sqrt{2}, \infty) \cap \Q
$$
does not admit a **lowest element** in $\Q$. We will make this more precise.
:::







## Axioms of Real Numbers

We now have all the key elements to introduce the Real Numbers $\R$. These ingredients are

- Definition of **field**
- Definition of **total order**
- The **Cut Property**

The definition of $\R$ is given in an axiomatic way.


::: Definition
### System of Real Numbers $\R$

A system of Real Numbers is a set $\R$ satisfying the following properties:

1. There is a relation $\leq$ of **total order** on $\R$, that is, they hold
    - (A1) Reflexivity: $\forall \, a \in \R$ 
    $$
    a \leq a \,,
    $$
    - (A2) Antisymmetry: It holds
    $$
    a \leq b \, \mbox{ and } \, b \leq a \,\, \implies \,\, a = b\,,
    $$
    - (A3) Transitivity: It holds
    $$
    a \leq b \,\, \mbox{ and } \,\, b \leq c \,\, \implies \,\, a = c \,,
    $$
    - (A4) Total order:  $\forall \, a,b \in \R$ we have 
    $$
    a \leq b \,\, \mbox{ or } \,\, b \leq a \,.
    $$

2. There is an operation $+$ of **sum** on $\R$ which associates to pairs $a,b \in \R$ the number $(a+b) \in \R$. The sum satisfies:
    - (B1) Commutativity: $\forall \, a,b \in \R$
    $$
    a+b = b+a
    $$
    - (B2) Associativity: $\forall \, a,b,c \in \R$
    $$
    (a+b)+c = a+(b+c) \,,
    $$
    - (B3) Additive Identity: $\exists \, 0 \in \R \st$
    $$ 
    a + 0 = 0 + a = a \,, \,\,\, \forall \, a \in \R\,,
    $$
    - (B4) Additive Inverse: $\forall$

:::









