::: {.content-hidden}
$
{{< include macros.tex >}}
$
:::





# Series



A series is the sum of all terms in a sequence:
$$
a_1 + a_2 + a_3 + \ldots + a_n + \ldots 
$$
Since we are dealing with an infinite amount of terms, we need to be careful.
For example, consider the series
$$
\sum_{k=1}^\infty (-1)^k = -1 + 1 - 1 + 1 - 1 + 1 - \ldots 
$${#eq-series-introduction}
If we sum the terms in pairs, we obtain
$$
\sum_{k=1}^\infty (-1)^k = (-1 + 1) + (- 1 + 1) + ( - 1 + 1) + \ldots  = 0\,.
$$
If we reorder the terms, we obtain a different result
\begin{align*}
\sum_{k=1}^\infty (-1)^k & = (1 + 1) - 1 + (1 + 1) - 1 + \ldots  \\
                         & = (2 - 1) + (2 - 1) + \ldots \\
                         & = 1 + 1 + \ldots \\
                         & = \infty \,. 
\end{align*}
Therefore commutativity of the sum does not hold when summing infinitely many terms. We need a good definition of convergence.


## Convergent series

We will develop the theory of series in for sequences in $\mathbb{C}$. All the results for complex series will also hold for series in $\mathbb{R}$. Some results will only hold for series in $\R$: this will be the case for comparison tests
in which the order relation of $\R$ is needed.


We start by defining partial sums.

::: Definition 
### Partial sums

Let $\left(a_{n}\right)_{n \in \mathbb{N}}$ be a sequence in $\mathbb{C}$. The $n$-th partial sum of $(a_n)$ is
$$
s_{n} :=a_{1}+a_{2}+\ldots+a_{n} = \sum_{k=1}^{n} a_{k}
$$
This sequence $\left(s_{n}\right)_{n \in \mathbb{N}}$ is called the sequence of **partial sums**.

:::

We can use the sequence of partial sums to define convergence of a series.


::: Definition 
### Convergent series

Let $\left(a_{n}\right)_{n \in \mathbb{N}}$ be a sequence in $\mathbb{C}$. We denote the series of $\left(a_{n}\right)_{n \in \mathbb{N}}$ by
$$
\sum_{k=1}^{\infty} a_{k}
$$
We say that this series **converges** to $s \in \mathbb{C}$ if
$$
\lim_{n \rightarrow \infty} \sum_{k=1}^{n} a_{k} = 
\lim_{n \rightarrow \infty} s_{n} = s \,.
$$
In this case we write
$$
\sum_{k=1}^{\infty} a_{k}=s \,.
$$

:::


::: Definition 
### Divergent series

Let $\left(a_{n}\right)_{n \in \mathbb{N}}$ be a sequence in $\mathbb{C}$. The series 
$$
\sum_{k=1}^\infty a_k 
$$
is **divergent** if the sequence of partial sums $(s_n)$ is divergent.

:::


::: Example 
Consider the series
$$
\sum_{k=1}^{\infty} \frac{1}{k(k+1)} \,.
$$
Note that
$$
\frac{1}{k(k+1)}=\frac{1}{k}-\frac{1}{k+1} \,.
$$
Hence, we can compute the partial sums $s_{n}$ as follows:
\begin{align*}
s_{n} & =\sum_{k=1}^{n} \frac{1}{k(k+1)} \\
& =\sum_{k=1}^{n}\left(\frac{1}{k}-\frac{1}{k+1}\right) \\
& =\frac{1}{1}-\frac{1}{2}+\frac{1}{2}-\frac{1}{3}+\frac{1}{3}-\frac{1}{4}+\ldots+\frac{1}{n}-\frac{1}{n+1} \\
& =1-\frac{1}{n+1} .
\end{align*}
Since,
$$
\lim_{n \rightarrow \infty} s_{n}=\lim _{n \rightarrow \infty}\left(1-\frac{1}{n+1}\right)=1 \,,
$$
the series converges to 1 , i.e.,
$$
\sum_{k=1}^{\infty} \frac{1}{k(k+1)}=1 \,.
$$
A series of this kind is called a **telescopic sum**, since we can *fold* the entire partial sum together, in such a way that only two terms remain.
:::

Let us go back to the series considered in (@eq-series-introduction).

::: Example 

Consider the series
$$
\sum_{k=1}^{\infty}(-1)^{k} \,.
$$
The partial sums $s_{n}$ are given by
$$
s_{n}=\sum_{k=1}^{n}(-1)^{k}= 
\begin{cases}-1 & \text { if } \, n \, \text { is odd }  \, \\ 
0 & \text { if } \, n  \, \text { is even. }\end{cases}
$$
Therefore $s_{n}$ diverges, so also the series diverges.

:::


In general, it is a difficult taks to compute the exact value of a series. Therefore, we will mainly focus our effort on determining whether a series converges or not. 

The following theorem shows that if the terms in the sequence do not converge to $0$, then the series cannot converge.

::: {.Theorem  #theorem-series-necessary}

Let $\left(a_{n}\right)_{n \in \mathbb{N}}$ be a sequence in $\mathbb{C}$. If the series 
$$
\sum_{k=1}^{\infty} a_{k} 
$$ 
converges, then 
$$
\lim_{k \rightarrow \infty} a_{k}=0 \,.
$$

:::

::: Proof

Suppose that 
$$
\sum_{k=1}^{\infty} a_{k}
$$ 
converges. By definition of convergent series there exists some $s \in \mathbb{C}$ such that
$$
\lim_{n \rightarrow \infty} s_{n}=\lim _{n \rightarrow \infty} \sum_{k=1}^{n} a_{k}=s \,.
$$
Note that then also
$$
\lim_{n \rightarrow \infty} s_{n+1}=s \,.
$$
Hence, by the Algebra of Limits in $\C$, we have that
$$
\lim_{n \rightarrow \infty}\left(s_{n+1}-s_{n}\right)=\lim _{n \rightarrow \infty} s_{n+1}-\lim _{n \rightarrow \infty} s_{n}=s-s=0 \,.
$$
Noting that 
$$
s_{n+1}-s_{n}=a_{n+1}\,,
$$ 
we obtain
$$
\lim _{n \rightarrow \infty} a_{n}=\lim _{n \rightarrow \infty} a_{n+1}=\lim _{n \rightarrow \infty}\left(s_{n+1}-s_{n}\right)=0 \, .
$$

:::



The contrapositive statement of Theorem \ref{theorem-series-necessary}
is particularly useful. For clarity, we give the precise statement. 



::: {.Theorem  #theorem-series-necessary-1}

Let $\left(a_{n}\right)_{n \in \mathbb{N}}$ be a sequence in $\mathbb{C}$. If 
$$
\lim_{k \rightarrow \infty} a_{k} \neq 0 \,,
$$
then the series
$$
\sum_{k=1}^{\infty} a_{k}
$$ 
does not converge.

:::





::: Example 

Consider the series
$$
\sum_{k=1}^\infty  (-1)^k \,.
$${#eq-example-series-1}
We have that
$$
\lim_{k \to \infty} a_k = \lim_{k \to \infty} (-1)^k  \neq 0 \,,
$$
being $a_k$ divergent. Therefore the series at (@eq-example-series-1) diverges
by Theorem \ref{theorem-series-necessary-1}.

:::


::: Example 
Consider the series
$$
\sum_{n=1}^{\infty} \frac{n}{5 n+11} \,.
$$
Then
$$
a_{n}:=\frac{n}{5 n+11}=\frac{1}{5 + \dfrac{11}{n} } \longrightarrow \frac{1}{5} \neq 0 \text {. }
$$
Hence, the series does not converge.
:::


::: Important

Theorem \ref{theorem-series-necessary-1} says that if $\sum_{k=1}^\infty a_k$ converges, 
then
$$
a_k \to 0 \,.
$$
In general the condition $a_k \to 0$ does not guarantee convergence of the 
associated series, as shown in the example below.

:::


::: Example

Consider the series
$$
\sum_{k=1}^\infty a_k \,, \quad a_k := \frac{1}{ \sqrt{k+1} + \sqrt{k} } \,.
$$
By the Algebra of Limits we have
$$
\lim_{k \to \infty} a_k = 0 \,.
$$
However the partial sums are given by
$$
s_n = \sum_{k=1}^n a_k = \sqrt{n+1} - 1 \,.
$$
Therefore $s_n$ is divergent and so the series is divergent.

> Exercise: Prove by induction that $\sum_{k=1}^n a_k = \sqrt{n+1} - 1$.

:::



::: Remark

It is customary to sum a series starting at $k=1$. However one could start
the sum from any $k=N$ with $N \in \N$. This would not affect the convergence
of the series, but of course it will change the value of the limit. 

:::


::: Example 

We have seen that 
$$
\sum_{k=1}^{\infty} \frac{1}{k(k+1)} = 1 \,.
$$
Hence also the series
$$
\sum_{k=7}^{\infty} \frac{1}{k(k+1)}
$$
converges. However, in this case, the partial sums are given by
\begin{align*}
s_{n} & =\sum_{k=7}^{n} \frac{1}{k(k+1)} \\
      & =\sum_{k=7}^{n}\left(\frac{1}{k}-\frac{1}{k+1}\right) \\
      & =\frac{1}{7}-\frac{1}{8}+\frac{1}{8}-\frac{1}{9}+\ldots+\frac{1}{n}-\frac{1}{n+1} \\
      & =\frac{1}{7}-\frac{1}{n+1} \,.
\end{align*}
Therefore
$$
\sum_{k=7}^{\infty} \frac{1}{k(k+1)}=\lim _{n \rightarrow \infty} s_{n}=\frac{1}{7} \,.
$$

:::



## Geometric series

